tmp

CoinClass.thy
@@ -1,20 +1,301 @@
 theory CoinClass imports "~~/src/HOL/Library/Multiset" begin
-
 type_alias val = nat
 
-locale coin =
+lemma finite_induct1[induct set: finite]:
+  assumes finite: "finite X"
+    and mem: "x \<in> X"
+    and base: "P {x}"
+    and step: "\<And>X x'. \<lbrakk> finite X; P X; x' \<notin> X; x \<in> X \<rbrakk> \<Longrightarrow> P (insert x' X)"
+  shows "P X"
+proof -
+  obtain X' where 1: "X = insert x X'" and 2: "x \<notin> X'" by (meson Set.set_insert mem)
+  have 3: "finite X'" using finite 1 by simp
+  show ?thesis
+  using 3 mem step[where ?X=X] unfolding 1 proof (induct rule: finite_induct)
+    case empty
+    show ?case using base .
+  next
+    case (insert x' F)
+    thus ?case
+    proof -
+      have "\<lbrakk> finite (insert x F); P (insert x F); x' \<notin> insert x F; x \<in> insert x F \<rbrakk> \<Longrightarrow> P (insert x' (insert x F))"
+        using step by blast
+      hence "P (insert x' (insert x F))" proof (cases "x = x'")
+        case True
+        thus ?thesis using insert.hyps(3) insert.prems(2) local.step by fastforce
+      next
+        case False
+        then show ?thesis using insert.hyps(1) insert.hyps(2) insert.hyps(3) insert.prems(2) local.step by force
+      qed
+      thus "P (insert x (insert x' F))" using insert_commute by metis
+    qed
+  qed
+qed
+
+locale wellorder_finite = finite + wellorder + order_bot
+begin
+
+definition suc :: "'a \<Rightarrow> 'a \<Rightarrow> bool"
+  where "suc a b \<equiv> less a b \<and> (\<nexists>c. less a c \<and> less c b)"
+
+lemma neq_botE:
+  assumes "a \<noteq> bot"
+  obtains b where "less b a" and "\<nexists>x. less b x \<and> less x a"
+proof (induct rule: less_induct)
+  case (less x)
+  then show ?case by (metis assms empty_iff bot_less finite infinite_growing lessThan_iff that)
+qed
+
+lemma
+  assumes base: "P bot"
+    and step: "\<And>x y. \<lbrakk> P x; suc x y \<rbrakk> \<Longrightarrow> P y"
+  shows "P x"
+proof (induct x rule: less_induct)
+  case (less x)
+  assume less_step: "\<And>y. less y x \<Longrightarrow> P y"
+  show ?case proof (cases "x = bot")
+    case True
+    show ?thesis unfolding True by (rule base)
+  next
+    case False
+    then obtain y where less: "less y x" and nex: "\<nexists>z. less y z \<and> less z x" using neq_botE by blast
+    have P: "P y" using less by (rule less_step)
+    have suc: "suc y x" unfolding suc_def using less nex by simp
+    show ?thesis using step P suc .
+  qed
+qed
+end
+
+locale ordering_bot = ordering +
+  fixes bot :: 'a ("\<bottom>")
+  assumes extremum[simp]: "\<And>x. less_eq bot x"
+
+locale semilattice_bot = semilattice_order_set + ordering_bot
+begin
+
+lemma finite_induct1_max:
+  fixes P :: "'a set \<Rightarrow> bool"
+  assumes finite: "finite X"
+    and bot_mem: "x \<in> X"
+    and base: "P {x}"
+    and extra: "Q X"
+    and extra_step: "\<And>X x'. Q (insert x' X) \<Longrightarrow> Q X"
+    and step: "\<And>X x'. \<lbrakk> finite X; P X; x' \<notin> X; x \<in> X; Q X\<rbrakk> \<Longrightarrow> P (insert x' X)"
+  shows "P X"
+using finite bot_mem extra proof (induct rule: finite_induct1)
+  show "x \<in> X" using bot_mem .
+next
+  show "P {x}" using base .
+next
+  fix X' :: "'a set" and x'
+  assume finite': "finite X'"
+    and imp_P_x: "\<lbrakk> x \<in> X'; Q X'\<rbrakk> \<Longrightarrow> P X'"
+    and nmem': "x' \<notin> X'"
+    and bot_mem_insert: "x \<in> insert x' X'"
+    and Q_insert: "Q (insert x' X')"
+  have Q_x': "Q X'" using extra_step Q_insert .
+  have "x = x' \<or> x \<in> X'" using bot_mem_insert by simp
+  thus "P (insert x' X')" proof
+    assume 1: "x \<in> X'"
+    have P_x': "P X'" using imp_P_x 1 Q_x' .
+    show "P (insert x' X')" using step finite' P_x' nmem' 1 Q_x' .
+  next
+    assume x_eq: "x = x'"
+    show "P (insert x' X')"
+    using finite' Q_x' Q_insert proof (induct rule: finite_induct)
+      case empty
+      show ?case using base unfolding x_eq .
+    next
+      case (insert x'' X'')
+      assume finite'': "finite X''"
+        and nmem'': "x'' \<notin> X''"
+        and imp_P_insert'_'': "\<lbrakk> Q X''; Q (insert x' X'') \<rbrakk> \<Longrightarrow> P (insert x' X'')"
+        and Q_insert''_'': "Q (insert x'' X'')"
+      have Q_x'': "Q X''" using extra_step Q_insert''_'' .
+      show ?case
+      using step[where ?X="insert x' X''" and ?x'=x''] proof (subst insert_commute)
+        assume 2: "\<lbrakk>finite (insert x' X''); P (insert x' X''); x'' \<notin> insert x' X''; x \<in> insert x' X''; Q (insert x' X'')\<rbrakk>
+     \<Longrightarrow> P (insert x'' (insert x' X''))"
+        show "P (insert x'' (insert x' X''))" proof (cases "x'' = x")
+          case True
+          have P_insert'_'': "P (insert x' X'')" using imp_P_insert'_'' Q_x'' Q_insert''_'' unfolding x_eq True .
+          show ?thesis using P_insert'_'' unfolding x_eq True by simp
+        next
+          case False
+          show ?thesis
+          proof (rule 2)
+            show "finite (insert x' X'')" using finite'' by simp
+          next
+            show "P (insert x' X'')" by (metis extra_step imp_P_insert'_'' insert.prems(2) insert_commute)
+          next
+            show "x'' \<notin> insert x' X''" using nmem'' False unfolding x_eq by simp
+          next
+            show "x \<in> insert x' X''" unfolding x_eq by simp
+          next
+            show "Q (insert x' X'')" by (metis extra_step insert.prems(2) insert_commute)
+          qed
+        qed
+      qed
+    qed
+  qed
+qed
+end
+
+locale coin = wellorder_finite +
   fixes val_unit :: "'a \<Rightarrow> val"
-    and coin1 :: 'a
-    and less_eq :: "'a \<Rightarrow> 'a \<Rightarrow> bool"
-    and less :: "'a \<Rightarrow> 'a \<Rightarrow> bool"
-  assumes less_eq_def: "less_eq x y \<longleftrightarrow> val_unit x \<le> val_unit y"
-    and less_def: "less x y \<longleftrightarrow> val_unit x < val_unit y"
-    and finite_coins: "finite (UNIV :: 'a set)"
-    and val_unit_coin1: "val_unit coin1 = 1"
+  assumes val_unit_coin1[simp]: "val_unit bot = 1"
     and inj_val_unit: "inj val_unit"
     and val_unit_gt_0: "\<And>v. v \<in> range val_unit \<Longrightarrow> v > 0"
     and dvd_val_units: "\<And>v1 v2. \<lbrakk> v1 \<in> range val_unit; v2 \<in> range val_unit; v1 < v2 \<rbrakk> \<Longrightarrow> v1 dvd v2"
 begin
+
+definition less_eq_coin :: "'a \<Rightarrow> 'a \<Rightarrow> bool"
+  where "less_eq_coin x y \<longleftrightarrow> val_unit x \<le> val_unit y"
+
+definition less_coin :: "'a \<Rightarrow> 'a \<Rightarrow> bool"
+  where "less_coin x y \<longleftrightarrow> val_unit x < val_unit y"
+
+sublocale wellorder less_eq_coin less_coin
+unfolding less_eq_coin_def less_coin_def proof
+  fix x y
+  have 1: "x \<noteq> y \<longleftrightarrow> val_unit x \<noteq> val_unit y" using inj_val_unit by (simp add: inj_eq)
+  thus "(val_unit x < val_unit y) = (val_unit x \<le> val_unit y \<and> \<not> val_unit y \<le> val_unit x)" unfolding 1 by auto
+next
+  fix a
+  show "val_unit a \<le> val_unit a" by simp
+next
+  fix a b
+  assume 1: "val_unit a \<le> val_unit b"
+    and 2: "val_unit b \<le> val_unit a"
+  have 3: "a = b \<longleftrightarrow> val_unit a = val_unit b" using inj_val_unit by (simp add: inj_eq)
+  show "a = b" unfolding 3 using 1 2 by simp
+next
+  fix a b c
+  assume 1: "val_unit a \<le> val_unit b"
+    and 2: "val_unit b \<le> val_unit c"
+  thus "val_unit a \<le> val_unit c" by simp
+next
+  fix x y
+  show "val_unit x \<le> val_unit y \<or> val_unit y \<le> val_unit x" by fastforce
+  fix P a
+  assume step: "(\<And>x. (\<And>y. val_unit y < val_unit x \<Longrightarrow> P y) \<Longrightarrow> P x)"
+  thus "P a" by (rule measure_induct_rule[where ?f=val_unit]; metis)
+qed
+
+definition next_coin_on :: "'a set \<Rightarrow> 'a rel"
+  where "next_coin_on C \<equiv> { (c, c') | c c'. c \<in> C \<and> c' \<in> C \<and> less_coin c c' \<and> (\<nexists>c''. c'' \<in> C \<and> less_coin c c'' \<and> less_coin c'' c')}"
+
+theorem next_coin_on_emptyE:
+  assumes "p \<in> next_coin_on {}"
+  shows "P"
+using assms unfolding next_coin_on_def by simp
+
+theorem next_coin_on_singletonE:
+  assumes "p \<in> next_coin_on {c0}"
+  shows "P"
+using assms unfolding next_coin_on_def by clarsimp
+
+theorem id_nmem_next_coin_on: "(c, c) \<notin> next_coin_on C"
+  unfolding next_coin_on_def by simp
+
+theorem coin1_nmem_next_coin_on: "(c, bot) \<notin> next_coin_on C"
+unfolding next_coin_on_def proof auto
+  assume less: "less_coin c bot"
+  have not_less: "\<not>less_coin c bot" using val_unit_gt_0 unfolding less_coin_def val_unit_coin1 by auto
+  show "\<exists>c''. less_coin c c'' \<and> c'' \<in> C \<and> less_coin c'' bot " using less not_less by simp
+qed
+
+theorem wf_next_coin_on:
+  shows "wf (next_coin_on X)"
+unfolding wf_def proof 
+
+
+theorem next_coin_on_uniq:
+  assumes "(c1, c2) \<in> next_coin_on C"
+    and "(c1, c3) \<in> next_coin_on C"
+  shows "c2 = c3"
+using assms unfolding next_coin_on_def by fastforce
+
+
+abbreviation next_coin :: "'a rel"
+  where "next_coin \<equiv> next_coin_on UNIV"
+
+theorem
+  fixes c :: 'a
+  assumes mem: "c \<in> X"
+    and Min: "c = Min X"
+  shows "(\<nexists>c'. (c, c') \<in> next_coin_on X) \<longleftrightarrow> c = Max X"
+using finite[where ?A=X] mem proof (induct rule: finite_induct1_max[where ?x=c])
+  case mem
+  show "c \<in> X" using assms(1) .
+next
+  case Min
+  show "c = Min X" using assms(2) .
+next
+  case singleton
+  show ?case proof
+next
+  case (insert X x')
+  have "\<And>c' X c. \<lbrakk> \<nexists>a. next_coin_on (insert c' X) c a; c' \<notin> X \<rbrakk> \<Longrightarrow> (\<nexists>a. next_coin_on X c a)"
+    unfolding next_coin_on_def by (metis (full_types) insert_iff local.dual_order.strict_trans local.less_irrefl)
+  hence 1: "\<nexists>c'. next_coin_on X c c'" using insert.prems(2) insert.hyps(3) .
+  have "c = local.Max X" using insert.hyps(2) using insert.hyps(4) 1 .
+  thus "c = local.Max (insert x' X)" 
+qed
+
+
+theorem Min_UNIV: "local.Min UNIV = coin1"
+  by (metis UNIV_I finite image_eqI less_eq_coin_def less_one linorder_class.not_le local.Min.coboundedI local.antisym val_unit_coin1 val_unit_gt_0)
+
+
+theorem next_coin_on_eq_None: 
+  assumes "c \<in> X"
+  shows "next_coin_on X c = None \<longleftrightarrow> c = local.Max X"
+proof
+  assume "next_coin_on X c = None"
+  hence 1: "\<And>c'. c' \<in> X \<Longrightarrow> less_eq_coin c' c" using less_eq_coin_def next_coin_on2 by presburger
+  show "c = Max X" using finite[where ?A=X] 1 proof (induct rule: finite_induct1[where ?x=c])
+    case mem
+    thus "c \<in> X" using assms by simp
+  next
+    case singleton
+    thus ?case by simp
+  next
+    case (insert X x')
+    then show ?case by (metis empty_not_insert insertCI local.Max.coboundedI local.Max_in local.antisym local.finite)
+  qed
+next
+  assume "c = Max X"
+  thus "next_coin_on X c = None"
+    by (metis less_eq_coin_def linorder_class.not_le local.Max.coboundedI local.finite next_coin_on1 not_None_eq)
+qed
+
+theorem next_coin_eq_None: "next_coin c = None \<longleftrightarrow> c = local.Max UNIV"
+proof
+  assume "next_coin c = None"
+  hence "\<And>c'. less_eq_coin c' c" by (simp add: next_coin2)
+  thus "c = local.Max UNIV" by (simp add: local.antisym)
+next
+  assume 1: "c = local.Max UNIV"
+  show "next_coin c = None"
+  proof (cases "next_coin c")
+    case None
+    then show ?thesis by simp
+  next
+    case (Some a)
+    hence "less_coin c a" using next_coin1 by (simp add: less_coin_def)
+    then show ?thesis using 1 using finite by auto
+  qed
+qed
+
+
+lemma next_coin_neq_Some_coin1: "next_coin c \<noteq> Some coin1"
+  by (metis less_one linorder_class.not_less next_coin_def next_coin_on1 preorder_class.order_refl rangeI val_unit_coin1 val_unit_gt_0)
+
+lemma disj_next_coin_on:
+  assumes "x \<in> X"
+  shows "(\<exists>x'. x' \<in> X \<and> next_coin_on X x = Some x') \<or> next_coin_on X x = None"
+  using next_coin_on1 by blast
 
 lemma val_unit_neq_0: "val_unit c \<noteq> 0"
   by (simp add: val_unit_gt_0)
@@ -29,13 +310,12 @@ lemma neq_coin1_implies_val_unit_gt_1:
   shows "val_unit c > 1"
 proof -
   have "\<nexists>c. val_unit c = 0" using val_unit_gt_0 by simp
-  thus "val_unit c > 1" using assms val_unit_eq_1_is_coin1 by (meson less_one linorder_cases)
+  thus "val_unit c > 1" using assms val_unit_eq_1_is_coin1 by (meson less_one nat_neq_iff)
 qed
 
 
 definition val :: "'a multiset \<Rightarrow> val" where
   "val C \<equiv> sum_mset (image_mset val_unit C)"
-
 
 lemma val_mempty: "val {#} = 0"
   by (simp add: val_def)
@@ -43,6 +323,21 @@ lemma val_mempty: "val {#} = 0"
 lemma val_add_mset:
   "val (add_mset c C) = val_unit c + val C"
   by (simp add: val_def)
+
+lemma val_plus:
+  "val (C1 + C2) = val C1 + val C2"
+  by (simp add: val_def)
+
+lemma val_sum:
+  assumes "finite m"
+  shows "val (sum f m) = sum (val \<circ> f) m"
+using assms proof (induct rule: finite_induct)
+  case empty
+  thus ?case by (simp add: val_mempty)
+next
+  case (insert x F)
+  then show ?case by (simp add: val_plus)
+qed
 
 lemma val_singleton: "val {#c#} = val_unit c"
   unfolding val_add_mset val_mempty by simp
@@ -64,7 +359,7 @@ lemma val_gt_0_eq_not_empty: "val C > 0 \<longleftrightarrow> C \<noteq> {#}"
   using val_mempty val_eq_0D by auto
 
 lemma val_only_coin1: "val {#coin1#} = 1"
-  by (simp add: val_unit_coin1 val_def)
+  by (simp add: val_def)
 
 lemma val_eq_1_is_only_one_coin1:
   assumes "val C = 1"
@@ -119,42 +414,333 @@ proof -
   assume 1: "\<And>C. \<lbrakk>v = val C; normal_form C\<rbrakk> \<Longrightarrow> thesis"
   show thesis oops
 
+definition normalize :: "val \<Rightarrow> 'a multiset"
+  where "normalize v \<equiv> sum
+  (\<lambda>c. replicate_mset (
+    case next_coin c of
+      None \<Rightarrow> v div (val_unit c) |
+      Some c' \<Rightarrow> (v mod (val_unit c')) div (val_unit c)
+  ) c) (UNIV :: 'a set)"
 
-theorem ex1_normal_form: "\<exists>!C. v = val C \<and> normal_form C"
-  oops
-
-lemma "\<lbrakk> v1 dvd v2; v1 * c1 + v2 * c2 = v1 * (c1 + c1') + v2 * (c2 - c2'); c2 \<ge> c2' \<rbrakk> \<Longrightarrow> c1 + c2 < c1 + c1' + c2 - c2'" for c1 :: nat
-  oops
-
-lemma "\<lbrakk> v1 * c1 + v2 * c2 = v1 * c1' + v2 * c2' \<rbrakk> \<Longrightarrow> c1 + c2 < c1' + c2'"
-  oops
-
-lemma "\<lbrakk> v1 dvd v2; c2 \<ge> c2' \<rbrakk> \<Longrightarrow> \<nexists>c1' c2'. v1 * c1 + v2 * c2 = v1 * (c1 + c1') + v2 * (c2 - c2')"
-  oops
-
-sublocale linorder less_eq less
-unfolding less_eq_def less_def proof
-  fix x y
-  have 1: "x \<noteq> y \<longleftrightarrow> val_unit x \<noteq> val_unit y" using inj_val_unit by (simp add: inj_eq)
-  thus "(val_unit x < val_unit y) = (val_unit x \<le> val_unit y \<and> \<not> val_unit y \<le> val_unit x)" unfolding 1 by auto
-next
-  fix a
-  show "val_unit a \<le> val_unit a" by simp
-next
-  fix a b
-  assume 1: "val_unit a \<le> val_unit b"
-    and 2: "val_unit b \<le> val_unit a"
-  have 3: "a = b \<longleftrightarrow> val_unit a = val_unit b" using inj_val_unit by (simp add: inj_eq)
-  show "a = b" unfolding 3 using 1 2 by simp
-next
-  fix a b c
-  assume 1: "val_unit a \<le> val_unit b"
-    and 2: "val_unit b \<le> val_unit c"
-  thus "val_unit a \<le> val_unit c" by simp
-next
-  fix x y
-  show "val_unit x \<le> val_unit y \<or> val_unit y \<le> val_unit x" by fastforce
+lemma normalize_0: "normalize 0 = {#}"
+unfolding normalize_def proof -
+  have 1: "\<And>c. 0 div val_unit c = 0" by simp
+  have 2: "\<And>c c'. 0 mod val_unit c' div val_unit c = 0" by simp
+  have 3: "\<And>c. (case next_coin c of None \<Rightarrow> 0 | _ \<Rightarrow> 0) = 0" by (simp add: option.case_eq_if)
+  show "sum (\<lambda>c. replicate_mset (case next_coin c of None \<Rightarrow> 0 div val_unit c | Some c' \<Rightarrow> 0 mod val_unit c' div val_unit c) c) UNIV = {#}"
+  unfolding 1 2 3 by simp
 qed
-end
 
+lemma normalize_val_unit: "normalize (val_unit c) = {# c #}"
+unfolding normalize_def proof -
+  have 1: "\<And>c'. next_coin c' = None \<Longrightarrow> val_unit c div val_unit c' = (if c = c' then 1 else 0)"
+  proof auto
+    assume "next_coin c = None"
+    hence "c = local.Max UNIV" using next_coin_eq_None by blast
+    have "val_unit c \<noteq> 0" using val_unit_gt_0 by auto
+    thus "val_unit c div val_unit c = Suc 0" by simp
+  next
+    fix c'
+    assume "next_coin c' = None" and neq: "c \<noteq> c'"
+    hence c'_eq: "c' = local.Max UNIV" using next_coin_eq_None by blast
+    hence "less_coin c (local.Max UNIV)"
+      by (metis UNIV_I finite local.Max.coboundedI local.antisym local.not_le neq)
+    thus "val_unit c div val_unit c' = 0" unfolding c'_eq less_coin_def by simp
+  qed
+  have 2: "\<And>c' c''. next_coin c' = Some c'' \<Longrightarrow> val_unit c mod val_unit c'' div val_unit c' = (if c = c' then 1 else 0)"
+  proof auto
+    fix c2
+    assume "next_coin c = Some c2"
+    hence "less_coin c c2" using next_coin1 by blast
+    hence "val_unit c mod val_unit c2 = val_unit c" unfolding less_coin_def by simp
+    thus "val_unit c mod val_unit c2 div val_unit c = Suc 0" using val_unit_neq_0[where ?c=c] by simp
+  next
+    fix c1 c2
+    assume 1: "next_coin c1 = Some c2"
+      and neq: "c \<noteq> c1"
+    show "val_unit c mod val_unit c2 div val_unit c1 = 0"
+    proof (cases "less_coin c2 c")
+      case True
+      hence "val_unit c2 dvd val_unit c" using dvd_val_units[where ?v1.0="val_unit c2" and ?v2.0="val_unit c"] next_coin1 by (simp add: less_coin_def)
+      hence "val_unit c mod val_unit c2 = 0" by simp
+      thus ?thesis by simp
+    next
+      case False
+      hence "val_unit c2 = val_unit c \<or> less_coin c c2" using antisym_conv3 by force
+      thus ?thesis unfolding less_coin_def proof (auto; cases "less_coin c c1")
+        case True
+        thus "val_unit c div val_unit c1 = 0" by (simp add: less_coin_def)
+      next
+        case False
+        hence 2: "less_coin c1 c" using neq by (meson less_coin_def local.not_less_iff_gr_or_eq)
+        assume 3: "val_unit c < val_unit c2"
+        have "\<nexists>c3. less_coin c1 c3 \<and> less_coin c3 c2" using 1 next_coin1 by blast
+        hence "False" using 2 3 by (simp add: less_coin_def)
+        thus "val_unit c div val_unit c1 = 0" by simp
+      qed
+    qed
+  qed
+  have 1: "\<And>ca. (case next_coin ca of None \<Rightarrow> val_unit c div val_unit ca | Some c' \<Rightarrow> val_unit c mod val_unit c' div val_unit ca) = (if c = ca then 1 else 0)"
+  proof -
+    fix ca :: 'a
+    show "(case next_coin ca of None \<Rightarrow> val_unit c div val_unit ca | Some c' \<Rightarrow> val_unit c mod val_unit c' div val_unit ca) = (if c = ca then 1 else 0)"
+    proof (cases "next_coin ca")
+      case None
+      thus ?thesis using 1 by simp
+    next
+      case (Some a)
+      thus ?thesis using 2 by simp
+    qed
+  qed
+  have 2: "UNIV = (UNIV - {c}) \<union> {c}" by blast
+  show "sum (\<lambda>ca. replicate_mset (case next_coin ca of None \<Rightarrow> val_unit c div val_unit ca | Some c' \<Rightarrow> val_unit c mod val_unit c' div val_unit ca) ca) UNIV = {#c#}"
+  unfolding 1 proof (subst 2)
+    have 3: "sum (\<lambda>ca. replicate_mset (if c = ca then 1 else 0) ca) (UNIV - {c} \<union> {c}) = sum (\<lambda>ca. replicate_mset (if c = ca then 1 else 0) ca) (UNIV - {c}) + sum (\<lambda>ca. replicate_mset (if c = ca then 1 else 0) ca) {c}"
+      by (metis (no_types, lifting) "2" Diff_UNIV Diff_eq_empty_iff finite sum.subset_diff)
+    show "sum (\<lambda>ca. replicate_mset (if c = ca then 1 else 0) ca) (UNIV - {c} \<union> {c}) = {#c#}"
+    unfolding 3 by simp
+  qed
+qed
+
+lemma sum_Un:
+  fixes f :: "'b \<Rightarrow> 'a multiset"
+  assumes "finite X" "finite Y"
+    and "disjnt X Y"
+  shows "sum f (X \<union> Y) = sum f X + sum f Y"
+  by (meson assms(1) assms(2) assms(3) disjnt_def sum.union_disjoint)
+
+lemma sum_subst:
+  fixes f :: "'b \<Rightarrow> 'a multiset"
+  assumes "\<And>y. \<lbrakk> y \<in> X; x \<noteq> y \<rbrakk> \<Longrightarrow> f y = g y"
+  shows "sum f (X - {x}) = sum g (X - {x})"
+  by (metis DiffD1 DiffD2 assms(1) singletonI sum.cong)
+
+lemma
+  assumes "Some c2 = next_coin coin1"
+    and "1 < v" "v < val_unit c2"
+  shows "normalize v = replicate_mset v coin1"
+unfolding normalize_def proof -
+  have 1: "UNIV = UNIV - {coin1} \<union> {coin1}" by blast
+  show "sum (\<lambda>c. replicate_mset (case next_coin c of None \<Rightarrow> v div val_unit c | Some c' \<Rightarrow> v mod val_unit c' div val_unit c) c) UNIV = replicate_mset v coin1"
+  proof (subst 1)
+    have 2: "sum (\<lambda>c. replicate_mset (case next_coin c of None \<Rightarrow> v div val_unit c | Some c' \<Rightarrow> v mod val_unit c' div val_unit c) c) (UNIV - {coin1} \<union> {coin1}) = sum (\<lambda>c. replicate_mset (case next_coin c of None \<Rightarrow> v div val_unit c | Some c' \<Rightarrow> v mod val_unit c' div val_unit c) c) (UNIV - {coin1}) + sum (\<lambda>c. replicate_mset (case next_coin c of None \<Rightarrow> v div val_unit c | Some c' \<Rightarrow> v mod val_unit c' div val_unit c) c) {coin1}"
+      by (rule sum_Un; simp)
+    show "sum (\<lambda>c. replicate_mset (case next_coin c of None \<Rightarrow> v div val_unit c | Some c' \<Rightarrow> v mod val_unit c' div val_unit c) c) (UNIV - {coin1} \<union> {coin1}) = replicate_mset v coin1"
+    unfolding 2 proof -
+      have 3: "\<And>c. c \<noteq> coin1 \<Longrightarrow> v < val_unit c"
+      proof -
+        fix c
+        assume neq1: "c \<noteq> coin1"
+        show "v < val_unit c"
+        proof (cases "c = c2")
+          case True
+          thus ?thesis using assms(3) by simp
+        next
+          case False
+          note neq2 = False
+          hence "\<nexists>c3. val_unit coin1 < val_unit c3 \<and> val_unit c3 < val_unit c2" using assms(1) next_coin1 less_coin_def by metis
+          thus ?thesis using neq1 neq2 using assms(3) neq_coin1_implies_val_unit_gt_1 val_unit_coin1 by fastforce
+        qed
+      qed
+      have 4: "\<And>c. c \<noteq> coin1 \<Longrightarrow> v div val_unit c = 0" using 3 by simp
+      have 5: "\<And>c c'. \<lbrakk> c \<noteq> coin1; Some c' = next_coin c \<rbrakk> \<Longrightarrow> v mod val_unit c' div val_unit c = 0"
+      proof -
+        fix c c'
+        assume neq: "c \<noteq> coin1" and x: "Some c' = next_coin c"
+        have neq': "c' \<noteq> coin1" using next_coin_neq_Some_coin1[where ?c=c] x by auto
+        have "v < val_unit c'" using 3 neq' by simp
+        hence 6: "v mod val_unit c' = v" by simp
+        have 7: "v < val_unit c" using 3 neq by simp
+        thus " v mod val_unit c' div val_unit c = 0" unfolding 6 using 7 by simp
+      qed
+      have "\<And>c. c \<noteq> coin1 \<Longrightarrow> (case next_coin c of None \<Rightarrow> v div val_unit c | Some c' \<Rightarrow> v mod val_unit c' div val_unit c) = 0" using 4 5 by (simp add: option.case_eq_if)
+      hence 8: "sum (\<lambda>c. replicate_mset (case next_coin c of None \<Rightarrow> v div val_unit c | Some c' \<Rightarrow> v mod val_unit c' div val_unit c) c) (UNIV - {coin1}) = {#}"
+        by simp
+      have "\<And>c. c = coin1 \<Longrightarrow> (case next_coin c of None \<Rightarrow> v div val_unit c | Some c' \<Rightarrow> v mod val_unit c' div val_unit c) = v"
+        by (simp add: assms(1)[symmetric] assms(3))
+      hence 9: "sum (\<lambda>c. replicate_mset (case next_coin c of None \<Rightarrow> v div val_unit c | Some c' \<Rightarrow> v mod val_unit c' div val_unit c) c) {coin1} = replicate_mset v coin1"
+       by simp
+      show "sum (\<lambda>c. replicate_mset (case next_coin c of None \<Rightarrow> v div val_unit c | Some c' \<Rightarrow> v mod val_unit c' div val_unit c) c) (UNIV - {coin1}) + sum (\<lambda>c. replicate_mset (case next_coin c of None \<Rightarrow> v div val_unit c | Some c' \<Rightarrow> v mod val_unit c' div val_unit c) c) {coin1} = replicate_mset v coin1"
+      unfolding 8 9 by simp
+    qed
+  qed
+qed
+
+lemma val_replicate_mset: "val (replicate_mset n c) = n * val_unit c"
+proof (induct n)
+  case 0
+  thus ?case by (simp add: val_mempty)
+next
+  case (Suc n)
+  thus ?case by (simp add: val_add_mset)
+qed
+
+lemma size_sum:
+  fixes f :: "'b \<Rightarrow> 'a multiset"
+  assumes "finite m"
+  shows "size (sum f m) = sum (size \<circ> f) m"
+using assms proof (induct rule: finite_induct)
+  case empty
+  thus ?case by simp
+next
+  case (insert x F)
+  thus ?case by simp
+qed
+
+
+lemma size_replicate_mset: "size (replicate_mset n c) = n"
+ by simp
+
+lemma card_UNIV_eq_1D:
+  assumes UNIV: "card (UNIV :: 'a set) = 1"
+  shows "next_coin coin1 = None"
+proof -
+  have 1: "\<And>X x. \<lbrakk> x \<in> X; card X = 1 \<rbrakk> \<Longrightarrow> X = {x}" using card_1_singletonE by blast
+  hence 2: "(UNIV::'a set) = {coin1}"
+  proof (rule_tac 1[where ?X1="UNIV :: 'a set" and ?x1=coin1])
+    show "coin1 \<in> UNIV" by simp
+  next
+    show "card (UNIV :: 'a set) = 1" using UNIV .
+  qed
+  show "next_coin coin1 = None" by (simp add: 2 next_coin_eq_None)
+qed
+
+lemma finite_induct1_max:
+  fixes X :: "'a set"
+  assumes finite: "finite X"
+    and mem: "x \<in> X"
+    and x_eq_Min: "x = Min X"
+    and base: "P {x}"
+    and step: "\<And>X x'. \<lbrakk> finite X; P X; x' \<notin> X; x \<in> X; x = Min X; \<And>x''. x'' \<in> X \<Longrightarrow> less_coin x'' x' \<rbrakk> \<Longrightarrow> P (insert x' X)"
+  shows "P X"
+proof -
+  obtain X' where X_eq: "X = insert x X'" and nmem: "x \<notin> X'" using Set.set_insert[OF mem] .
+  have finite': "finite X'" using X_eq finite by simp
+  show ?thesis
+  using finite' mem x_eq_Min nmem unfolding X_eq proof (induct rule: finite_linorder_max_induct[where ?A=X'])
+    case empty
+    show ?case using base .
+  next
+    case (insert x' X)
+    assume finite': "finite X"
+      and step': "\<lbrakk>x \<in> insert x X; x = Min (insert x X); x \<notin> X\<rbrakk> \<Longrightarrow> P (insert x X)"
+      and nmem: "x \<notin> insert x' X"
+      and less_all: "\<forall>x'' \<in> X. less_coin x'' x'"
+      and Min: "x = Min (insert x (insert x' X))"
+    have x_eq: "x = Min (insert x X)"
+    proof -
+      have 1: "finite (insert x (insert x' X))" using finite' by simp
+      have 2: "x \<noteq> x'" using nmem by blast
+      have 3: "x = Min (insert x (insert x' X) - {x'})"
+      proof -
+        have Min_subI: "\<And>X x y. \<lbrakk> finite X; x = Min X; x \<noteq> y \<rbrakk> \<Longrightarrow> x = Min (X - {y})"
+        proof -
+          fix X :: "'a set" and x y :: 'a
+          assume finite: "finite X"
+            and x_eq: "x = Min X"
+            and x_neq: "x \<noteq> y"
+          show "x = Min (X - {y})"
+          proof (cases "y \<in> X")
+            case True
+            then show ?thesis using local.Min.remove local.finite_code local.min_def x_eq x_neq by presburger
+          next
+            case False
+            then show ?thesis by (simp add: x_eq)
+          qed
+        qed
+        show "x = Min (insert x (insert x' X) - {x'})" using Min_subI[where ?X1="insert x (insert x' X)" and ?x1=x and ?y1=x'] 1 Min 2 .
+      qed
+      have 4: "insert x (insert x' X) - {x'} = insert x X" using less_all nmem by fastforce
+      show "x = Min (insert x X)" using 3 unfolding 4 .
+    qed
+    show ?case
+    using step proof (subst insert_commute; rule meta_mp[where P="True"])
+      show "finite (insert x X)" using finite' by blast
+    next
+      show "P (insert x X)"
+      using step' proof (rule meta_mp; simp)
+      next
+        show "x = Min (insert x X)" using x_eq .
+      next
+        show "x \<notin> X" using nmem by blast
+      qed
+    next
+      show "x' \<notin> insert x X" using nmem less_all by fastforce
+    next
+      show "x \<in> insert x X" by simp
+    next
+      show "x = Min (insert x X)" using x_eq .
+    next
+      fix x''
+      assume "x'' \<in> insert x X"
+      thus "less_coin x'' x'" by (metis Min Min_le finite' finite_insert insert_iff less_all less_le nmem)
+    next
+      show True by simp
+    qed
+  qed
+qed
+
+
+lemma val_normalize: "val (normalize v) = v"
+unfolding normalize_def proof (simp add: val_sum val_replicate_mset)
+  show "(\<Sum>x\<in>UNIV. (case next_coin x of None \<Rightarrow> v div val_unit x | Some c' \<Rightarrow> v mod val_unit c' div val_unit x) * val_unit x) = v"
+  unfolding next_coin_def
+  using finite proof (induct arbitrary: v rule: finite_induct1_max[where ?x=coin1])
+    show "finite (UNIV::'a set)" using finite .
+  next
+    show "coin1 \<in> UNIV" by simp
+  next
+    show "coin1 = Min UNIV" using Min_UNIV by force
+  next
+    fix v
+    have 1: "next_coin_on {coin1} coin1 = None" using next_coin_on_eq_None by fastforce
+    show "(\<Sum>x\<in>{coin1}. (case next_coin_on {coin1} x of None \<Rightarrow> v div val_unit x | Some c' \<Rightarrow> v mod val_unit c' div val_unit x) * val_unit x) = v"
+      by (simp add: 1)
+  next
+    fix X x' v
+    assume "\<And>v. (\<And>x :: 'a set. finite x) \<Longrightarrow> (\<Sum>x\<in>X. (case next_coin_on X x of None \<Rightarrow> v div val_unit x | Some c' \<Rightarrow> v mod val_unit c' div val_unit x) * val_unit x) = v"
+    hence step: "\<And>v. (\<Sum>x\<in>X. (case next_coin_on X x of None \<Rightarrow> v div val_unit x | Some c' \<Rightarrow> v mod val_unit c' div val_unit x) * val_unit x) = v"
+    proof
+      fix v and x :: "'a set"
+      show "finite x" using finite .
+    next
+      fix v :: val
+      show "v = v" by (rule refl)
+    qed
+    assume nmem: "x' \<notin> X"
+      and mem: "coin1 \<in> X"
+      and coin1_eq: "coin1 = Min X"
+      and upper_bound: "\<And>x''. x'' \<in> X \<Longrightarrow> less_coin x'' x'"
+    have 1: "finite (insert x' X)" using finite .
+    have "x' = Max (insert x' X)" using upper_bound by (simp add: local.Max_insert2 local.dual_order.order_iff_strict)
+    hence 2: "next_coin_on (insert x' X) x' = None" using next_coin_on_eq_None by force
+    show "(\<Sum>x\<in>insert x' X. (case next_coin_on (insert x' X) x of None \<Rightarrow> v div val_unit x | Some c' \<Rightarrow> v mod val_unit c' div val_unit x) * val_unit x) = v"
+    using finite[where ?A=X] nmem proof (simp add: 2)
+      obtain y where y_eq: "y = Max X" and "y \<in> X" using mem by (metis empty_iff local.Max_in local.finite)
+      have "\<And>z. z \<noteq> y \<Longrightarrow> next_coin_on (insert x' X) z = next_coin_on X z" 
+      show "v div val_unit x' * val_unit x' +
+      (\<Sum>x\<in>X. (case next_coin_on (insert x' X) x of None \<Rightarrow> v div val_unit x | Some c' \<Rightarrow> v mod val_unit c' div val_unit x) * val_unit x) = v"
+    oops
+
+theorem normal_form_normalize: "normal_form (normalize v)"
+unfolding normal_form_def normalize_def proof auto
+  fix C'
+  assume "val (sum (\<lambda>c. replicate_mset (case next_coin c of None \<Rightarrow> v div val_unit c | Some c' \<Rightarrow> v mod val_unit c' div val_unit c) c) UNIV) = val C'"
+  hence "sum (\<lambda>c. (case next_coin c of None \<Rightarrow> v div val_unit c | Some c' \<Rightarrow> v mod val_unit c' div val_unit c) * val_unit c) UNIV = val C'"
+    by (metis (mono_tags, lifting) coin.val_sum coin_axioms comp_apply finite sum.cong val_replicate_mset)
+  thus "size (sum (\<lambda>c. replicate_mset (case next_coin c of None \<Rightarrow> v div val_unit c | Some c' \<Rightarrow> v mod val_unit c' div val_unit c) c) UNIV) \<le> size C'"
+  using finite proof (simp add: size_sum)    
+    assume "sum (\<lambda>c. (case next_coin c of None \<Rightarrow> v div val_unit c | Some c' \<Rightarrow> v mod val_unit c' div val_unit c) * val_unit c) UNIV = val C'"
+    show "sum (\<lambda>c. (case next_coin c of None \<Rightarrow> v div val_unit c | Some c' \<Rightarrow> v mod val_unit c' div val_unit c)) UNIV \<le> size C'"
+  oops
+
+theorem ex_normal_form:
+  fixes v :: val
+  assumes "normal_form Otsuri"
+    and "val Watasu \<ge> v"
+    and "Watasu \<subseteq># Saifu"
+  obtains Watasu where "normal_form (Saifu - Watasu + normalize (val Watasu - v))"
+  by (metis add.left_neutral cancel_comm_monoid_add_class.diff_cancel normal_form_normalize)
+
+end
 end
