Yen.thy
@@ -4,13 +4,21 @@ theory Yen imports CoinClass begin
 
 datatype Yen = One | Five | Ten | Fifty | Hundred | FiveHundreds
 
-fun Yen_unit :: "Yen \<Rightarrow> val" where
-  "Yen_unit One = 1" |
-  "Yen_unit Five = 5" |
-  "Yen_unit Ten = 10" |
-  "Yen_unit Fifty = 50" |
-  "Yen_unit Hundred = 100" |
-  "Yen_unit FiveHundreds = 500"
+fun Yen_unit :: "Yen \<Rightarrow> val"
+  where "Yen_unit One = 1"
+      | "Yen_unit Five = 5"
+      | "Yen_unit Ten = 10"
+      | "Yen_unit Fifty = 50"
+      | "Yen_unit Hundred = 100"
+      | "Yen_unit FiveHundreds = 500"
+
+fun Yen_next :: "Yen \<Rightarrow> Yen option"
+  where "Yen_next One = Some Five"
+      | "Yen_next Five = Some Ten"
+      | "Yen_next Ten = Some Fifty"
+      | "Yen_next Fifty = Some Hundred"
+      | "Yen_next Hundred = Some FiveHundreds"
+      | "Yen_next FiveHundreds = None"
 
 theorem Yen_UNIV_eq: "UNIV = {One, Five, Ten, Fifty, Hundred, FiveHundreds}"
 proof (rule equalityI; rule subsetI)
@@ -21,13 +29,7 @@ next
   show "x \<in> UNIV" by simp
 qed
 
-definition less_eq_Yen :: "Yen \<Rightarrow> Yen \<Rightarrow> bool"
-  where "less_eq_Yen y1 y2 \<equiv> Yen_unit y1 \<le> Yen_unit y2"
-
-definition less_Yen :: "Yen \<Rightarrow> Yen \<Rightarrow> bool"
-  where "less_Yen y1 y2 \<equiv> Yen_unit y1 < Yen_unit y2"
-
-interpretation Yen: coin Yen_unit One less_eq_Yen less_Yen
+interpretation Yen: coin Yen_unit One Yen_next
 proof
   show "finite (UNIV::Yen set)"
   unfolding Yen_UNIV_eq by simp
@@ -67,10 +69,53 @@ next
   assume "v1 \<in> range Yen_unit" "v2 \<in> range Yen_unit" "v1 < v2"
   thus "v1 dvd v2" unfolding Yen_UNIV_eq by fastforce
 next
-  fix x y
-  show "less_eq_Yen x y = (Yen_unit x \<le> Yen_unit y)" unfolding less_eq_Yen_def by simp
+  fix c1 c2
+  assume 1: "Yen_next c1 = Some c2"
+  thus "Yen_unit c1 < Yen_unit c2 \<and> (\<nexists>c3. Yen_unit c3 < Yen_unit c2 \<and> Yen_unit c1 < Yen_unit c3)" 
+  proof (rule_tac Yen.exhaust[where ?y=c1]; auto)
+    fix c3
+    assume "Yen_unit c3 < 5" "Suc 0 < Yen_unit c3"
+    thus False by (rule_tac Yen.exhaust[where ?y=c3]; simp)
+  next
+    fix c3
+    assume "Yen_unit c3 < 10" "5 < Yen_unit c3"
+    thus False by (rule_tac Yen.exhaust[where ?y=c3]; simp)
+  next
+    fix c3
+    assume "Yen_unit c3 < 50" "10 < Yen_unit c3"
+    thus False by (rule_tac Yen.exhaust[where ?y=c3]; simp)
+  next
+    fix c3
+    assume "Yen_unit c3 < 100" "50 < Yen_unit c3"
+    thus False by (rule_tac Yen.exhaust[where ?y=c3]; simp)
+  next
+    fix c3
+    assume "Yen_unit c3 < 500" "100 < Yen_unit c3"
+    thus False by (rule_tac Yen.exhaust[where ?y=c3]; simp)
+  qed
 next
-  fix x y
-  show "less_Yen x y = (Yen_unit x < Yen_unit y)" unfolding less_Yen_def by simp
+  fix c1 c2
+  assume "Yen_next c1 = None"
+  thus "Yen_unit c2 \<le> Yen_unit c1" by (rule_tac Yen.exhaust[where ?y=c1]; simp; rule_tac Yen.exhaust[where ?y=c2]; simp)
 qed
+
+lemma max_FiveHundreds: "Yen.max c FiveHundreds = FiveHundreds"
+  by (rule Yen.exhaust[where ?y=c]; simp add: Yen.max_def Yen.less_eq_coin_def)
+
+theorem "Yen.Min UNIV = One"
+  by (rule Yen.Min_UNIV)
+
+theorem "Yen.Max UNIV = FiveHundreds"
+proof -
+  have "Yen.Max UNIV = Yen.Max {One, Five, Ten, Fifty, Hundred, FiveHundreds}" unfolding Yen_UNIV_eq by (rule refl)
+  also have "... = Yen.max One (Yen.Max {Five, Ten, Fifty, Hundred, FiveHundreds})" by simp
+  also have "... = Yen.max One (Yen.max Five (Yen.Max {Ten, Fifty, Hundred, FiveHundreds}))" by simp
+  also have "... = Yen.max One (Yen.max Five (Yen.max Ten (Yen.Max {Fifty, Hundred, FiveHundreds})))" by simp
+  also have "... = Yen.max One (Yen.max Five (Yen.max Ten (Yen.max Fifty (Yen.Max {Hundred, FiveHundreds}))))" by simp
+  also have "... = Yen.max One (Yen.max Five (Yen.max Ten (Yen.max Fifty (Yen.max Hundred FiveHundreds))))" by simp
+  also have "... = FiveHundreds" by (simp add: max_FiveHundreds)
+  ultimately show "Yen.Max UNIV = ..." by simp
+qed
+
+
 end
